RSL protocol and safety proof => Dafny 3.0.0

ironfleet/src/Dafny/Distributed/Services/RSL/AbstractService.s.dfy
@@ -26,60 +26,60 @@ datatype AppRequest = AppRequest(client:EndPoint, seqno:int, request:AppMessage)
 datatype AppReply   = AppReply(client:EndPoint, seqno:int, reply:AppMessage)
 
 datatype ServiceState' = ServiceState'(
-    serverAddresses:set<EndPoint>,
-    app:AppState,
-    requests:set<AppRequest>,
-    replies:set<AppReply>
-    )
+  serverAddresses:set<EndPoint>,
+  app:AppState,
+  requests:set<AppRequest>,
+  replies:set<AppReply>
+  )
 
 type ServiceState = ServiceState'
 
 predicate Service_Init(s:ServiceState, serverAddresses:set<EndPoint>)
 {
-       s.serverAddresses == serverAddresses
-    && s.app == AppInitialize()
-    && s.requests == {}
-    && s.replies == {}
+  && s.serverAddresses == serverAddresses
+  && s.app == AppInitialize()
+  && s.requests == {}
+  && s.replies == {}
 }
 
 predicate ServiceExecutesAppRequest(s:ServiceState, s':ServiceState, req:AppRequest)
 {
-       s'.serverAddresses == s.serverAddresses
-    && s'.requests == s.requests + { req }
-    && s'.app == AppHandleRequest(s.app, req.request).0
-    && s'.replies == s.replies + { AppReply(req.client, req.seqno, AppHandleRequest(s.app, req.request).1) }
+  && s'.serverAddresses == s.serverAddresses
+  && s'.requests == s.requests + { req }
+  && s'.app == AppHandleRequest(s.app, req.request).0
+  && s'.replies == s.replies + { AppReply(req.client, req.seqno, AppHandleRequest(s.app, req.request).1) }
 }
 
 predicate StateSequenceReflectsBatchExecution(s:ServiceState, s':ServiceState, intermediate_states:seq<ServiceState>, batch:seq<AppRequest>)
 {
-       |intermediate_states| == |batch| + 1
-    && intermediate_states[0] == s
-    && last(intermediate_states) == s'
-    && forall i :: 0 <= i < |batch| ==> ServiceExecutesAppRequest(intermediate_states[i], intermediate_states[i+1], batch[i])
+  && |intermediate_states| == |batch| + 1
+  && intermediate_states[0] == s
+  && last(intermediate_states) == s'
+  && forall i :: 0 <= i < |batch| ==> ServiceExecutesAppRequest(intermediate_states[i], intermediate_states[i+1], batch[i])
 }
 
 predicate Service_Next(s:ServiceState, s':ServiceState)
 {
-    exists intermediate_states, batch :: StateSequenceReflectsBatchExecution(s, s', intermediate_states, batch)
+  exists intermediate_states, batch :: StateSequenceReflectsBatchExecution(s, s', intermediate_states, batch)
 }
 
 function Uint64ToBytes(u:uint64) : seq<byte>
 {
-    [byte( u/0x1000000_00000000),
-     byte((u/  0x10000_00000000)%0x100),
-     byte((u/    0x100_00000000)%0x100),
-     byte((u/      0x1_00000000)%0x100),
-     byte((u/         0x1000000)%0x100),
-     byte((u/           0x10000)%0x100),
-     byte((u/             0x100)%0x100),
-     byte( u                    %0x100)]
+  [( u/0x1000000_00000000)        as byte,
+   ((u/  0x10000_00000000)%0x100) as byte,
+   ((u/    0x100_00000000)%0x100) as byte,
+   ((u/      0x1_00000000)%0x100) as byte,
+   ((u/         0x1000000)%0x100) as byte,
+   ((u/           0x10000)%0x100) as byte,
+   ((u/             0x100)%0x100) as byte,
+   ( u                    %0x100) as byte]
 }
 
 function MarshallServiceRequest(seqno:int, request:AppMessage) : seq<byte>
 {
   if 0 <= seqno < 0x1_0000_0000_0000_0000 then
         [ 0, 0, 0, 0, 0, 0, 0, 0] // MarshallMesssage_Request magic number
-      + Uint64ToBytes(uint64(seqno))        
+      + Uint64ToBytes(seqno as uint64)        
       + MarshallAppMessage(request)
   else 
       [ 1 ]
@@ -88,20 +88,20 @@ function MarshallServiceRequest(seqno:int, request:AppMessage) : seq<byte>
 function MarshallServiceReply(seqno:int, reply:AppMessage) : seq<byte>
 {
   if 0 <= seqno < 0x1_0000_0000_0000_0000 then
-        [ 0, 0, 0, 0, 0, 0, 0, 6] // MarshallMesssage_Reply magic number
-      + Uint64ToBytes(uint64(seqno))        
-      + MarshallAppMessage(reply)
+      [ 0, 0, 0, 0, 0, 0, 0, 6] // MarshallMesssage_Reply magic number
+    + Uint64ToBytes(seqno as uint64)        
+    + MarshallAppMessage(reply)
   else 
-      [ 1 ]
+    [ 1 ]
 }
 
 predicate Service_Correspondence(concretePkts:set<LPacket<EndPoint, seq<byte>>>, serviceState:ServiceState) 
 {
-       (forall p, seqno, reply :: p in concretePkts && p.src in serviceState.serverAddresses && p.msg == MarshallServiceReply(seqno, reply) ==>
-               AppReply(p.dst, seqno, reply) in serviceState.replies)
-    && (forall req :: req in serviceState.requests ==> exists p :: p in concretePkts && p.dst in serviceState.serverAddresses 
-                                                                && p.msg == MarshallServiceRequest(req.seqno, req.request)
-                                                                && p.src == req.client)
+  && (forall p, seqno, reply :: p in concretePkts && p.src in serviceState.serverAddresses && p.msg == MarshallServiceReply(seqno, reply) ==>
+             AppReply(p.dst, seqno, reply) in serviceState.replies)
+  && (forall req :: req in serviceState.requests ==> exists p :: p in concretePkts && p.dst in serviceState.serverAddresses 
+                                                                    && p.msg == MarshallServiceRequest(req.seqno, req.request)
+                                                                    && p.src == req.client)
 }
 
 }
