ironfleet/src/Dafny/Distributed/Protocol/RSL/CommonProof/MaxBallot.i.dfy
@@ -7,104 +7,106 @@ include "MaxBallotISent1a.i.dfy"
 
 module CommonProof__MaxBallot_i {
 import opened LiveRSL__DistributedSystem_i
+import opened LiveRSL__Constants_i
+import opened LiveRSL__Types_i
 import opened CommonProof__Assumptions_i
 import opened CommonProof__Constants_i
 import opened CommonProof__Actions_i
 import opened CommonProof__PacketSending_i
 import opened CommonProof__MaxBallotISent1a_i
+import opened Temporal__Temporal_s
 
 lemma lemma_MaxBalLeqMaxBallotPrimarySent1a(
-    b:Behavior<RslState>,
-    c:LConstants,
-    i:int,
-    idx:int
-    )
-    requires IsValidBehaviorPrefix(b, c, i);
-    requires 0 <= i;
-    requires 0 <= idx < |b[i].replicas|;
-    ensures  0 <= b[i].replicas[idx].replica.acceptor.max_bal.proposer_id < |b[i].replicas|;
-    ensures  var max_bal := b[i].replicas[idx].replica.acceptor.max_bal;
-             BalLeq(max_bal, b[i].replicas[max_bal.proposer_id].replica.proposer.max_ballot_i_sent_1a);
-    decreases i;
+  b:Behavior<RslState>,
+  c:LConstants,
+  i:int,
+  idx:int
+  )
+  requires IsValidBehaviorPrefix(b, c, i)
+  requires 0 <= i
+  requires 0 <= idx < |b[i].replicas|
+  ensures  0 <= b[i].replicas[idx].replica.acceptor.max_bal.proposer_id < |b[i].replicas|
+  ensures  var max_bal := b[i].replicas[idx].replica.acceptor.max_bal;
+           BalLeq(max_bal, b[i].replicas[max_bal.proposer_id].replica.proposer.max_ballot_i_sent_1a)
+  decreases i
 {
-    if i > 0
+  if i > 0
+  {
+    lemma_ConstantsAllConsistent(b, c, i-1);
+    lemma_ConstantsAllConsistent(b, c, i);
+    lemma_AssumptionsMakeValidTransition(b, c, i-1);
+
+    var s := b[i-1].replicas[idx].replica;
+    var s' := b[i].replicas[idx].replica;
+    var max_bal := s.acceptor.max_bal;
+    var max_bal' := s'.acceptor.max_bal;
+
+    if max_bal == max_bal'
     {
-        lemma_ConstantsAllConsistent(b, c, i-1);
-        lemma_ConstantsAllConsistent(b, c, i);
-        lemma_AssumptionsMakeValidTransition(b, c, i-1);
-
-        var s := b[i-1].replicas[idx].replica;
-        var s' := b[i].replicas[idx].replica;
-        var max_bal := s.acceptor.max_bal;
-        var max_bal' := s'.acceptor.max_bal;
-
-        if max_bal == max_bal'
-        {
-            lemma_MaxBalLeqMaxBallotPrimarySent1a(b, c, i-1, idx);
-            lemma_MaxBallotISent1aMonotonicOneStep(b, c, i-1, max_bal.proposer_id);
-        }
-        else
-        {
-            var ios := lemma_ActionThatChangesReplicaIsThatReplicasAction(b, c, i-1, idx);
-            var nextActionIndex := b[i-1].replicas[idx].nextActionIndex;
-            assert nextActionIndex == 0;
-            var p := ios[0].r;
-            lemma_PacketProcessedImpliesPacketSent(b[i-1], b[i], idx, ios, p);
-            assert p in b[i-1].environment.sentPackets;
-            if p.msg.RslMessage_1a?
-            {
-                lemma_Message1aLeqMaxBallotSenderSent1a(b, c, i-1, p);
-            }
-            else if p.msg.RslMessage_2a?
-            {
-                lemma_Message2aLeqMaxBallotSenderSent1a(b, c, i-1, p);
-            }
-            else
-            {
-                assert false;
-            }
-        }
+      lemma_MaxBalLeqMaxBallotPrimarySent1a(b, c, i-1, idx);
+      lemma_MaxBallotISent1aMonotonicOneStep(b, c, i-1, max_bal.proposer_id);
     }
+    else
+    {
+      var ios := lemma_ActionThatChangesReplicaIsThatReplicasAction(b, c, i-1, idx);
+      var nextActionIndex := b[i-1].replicas[idx].nextActionIndex;
+      assert nextActionIndex == 0;
+      var p := ios[0].r;
+      lemma_PacketProcessedImpliesPacketSent(b[i-1], b[i], idx, ios, p);
+      assert p in b[i-1].environment.sentPackets;
+      if p.msg.RslMessage_1a?
+      {
+        lemma_Message1aLeqMaxBallotSenderSent1a(b, c, i-1, p);
+      }
+      else if p.msg.RslMessage_2a?
+      {
+        lemma_Message2aLeqMaxBallotSenderSent1a(b, c, i-1, p);
+      }
+      else
+      {
+        assert false;
+      }
+    }
+  }
 }
 
 lemma lemma_VotePrecedesMaxBal(
-    b:Behavior<RslState>,
-    c:LConstants,
-    i:int,
-    idx:int,
-    opn:OperationNumber
-    )
-    requires IsValidBehaviorPrefix(b, c, i);
-    requires 0 <= i;
-    requires 0 <= idx < |b[i].replicas|;
-    requires opn in b[i].replicas[idx].replica.acceptor.votes;
-    ensures  BalLeq(b[i].replicas[idx].replica.acceptor.votes[opn].max_value_bal, b[i].replicas[idx].replica.acceptor.max_bal);
-    decreases i;
+  b:Behavior<RslState>,
+  c:LConstants,
+  i:int,
+  idx:int,
+  opn:OperationNumber
+  )
+  requires IsValidBehaviorPrefix(b, c, i)
+  requires 0 <= i
+  requires 0 <= idx < |b[i].replicas|
+  requires opn in b[i].replicas[idx].replica.acceptor.votes
+  ensures  BalLeq(b[i].replicas[idx].replica.acceptor.votes[opn].max_value_bal, b[i].replicas[idx].replica.acceptor.max_bal)
+  decreases i
 {
-    if i == 0
-    {
-        return;
-    }
+  if i == 0
+  {
+    return;
+  }
 
-    lemma_ReplicaConstantsAllConsistent(b, c, i, idx);
-    lemma_ReplicaConstantsAllConsistent(b, c, i-1, idx);
-    lemma_AssumptionsMakeValidTransition(b, c, i-1);
+  lemma_ReplicaConstantsAllConsistent(b, c, i, idx);
+  lemma_ReplicaConstantsAllConsistent(b, c, i-1, idx);
+  lemma_AssumptionsMakeValidTransition(b, c, i-1);
 
-    var s := b[i-1].replicas[idx].replica.acceptor;
-    var s' := b[i].replicas[idx].replica.acceptor;
+  var s := b[i-1].replicas[idx].replica.acceptor;
+  var s' := b[i].replicas[idx].replica.acceptor;
 
-    if s' == s
-    {
-        lemma_VotePrecedesMaxBal(b, c, i-1, idx, opn);
-        return;
-    }
+  if s' == s
+  {
+    lemma_VotePrecedesMaxBal(b, c, i-1, idx, opn);
+    return;
+  }
 
-    var ios := lemma_ActionThatChangesReplicaIsThatReplicasAction(b, c, i-1, idx);
-    if opn in s.votes
-    {
-        lemma_VotePrecedesMaxBal(b, c, i-1, idx, opn);
-    }
-     
+  var ios := lemma_ActionThatChangesReplicaIsThatReplicasAction(b, c, i-1, idx);
+  if opn in s.votes
+  {
+    lemma_VotePrecedesMaxBal(b, c, i-1, idx, opn);
+  }
 }
 
 }
