ironfleet/src/Dafny/Distributed/Protocol/RSL/CommonProof/ReplyCache.i.dfy
@@ -10,91 +10,101 @@ include "PacketSending.i.dfy"
 
 module CommonProof__ReplyCache_i {
 
+import opened LiveRSL__Constants_i
 import opened LiveRSL__DistributedSystem_i
+import opened LiveRSL__Environment_i
+import opened LiveRSL__Message_i
+import opened LiveRSL__Replica_i
+import opened LiveRSL__Types_i
+import opened Concrete_NodeIdentity_i
 import opened CommonProof__Assumptions_i
 import opened CommonProof__Actions_i
+import opened CommonProof__Constants_i
 import opened CommonProof__PacketSending_i
+import opened Temporal__Temporal_s
+import opened Environment_s
 
 predicate ReplyCacheObjectInv(cache:ReplyCache, client:NodeIdentity)
 {
-    client in cache ==> cache[client].Reply? && cache[client].client == client
+  client in cache ==> cache[client].Reply? && cache[client].client == client
 }
 
 predicate ReplyCacheStateInv(ps:RslState, client:NodeIdentity)
 {
-       (forall p :: p in ps.environment.sentPackets && p.src in ps.constants.config.replica_ids && p.msg.RslMessage_AppStateSupply? ==>
-        ReplyCacheObjectInv(p.msg.reply_cache, client))
-    && (forall idx :: 0 <= idx < |ps.replicas| ==> ReplyCacheObjectInv(ps.replicas[idx].replica.executor.reply_cache, client))
+  && (forall p :: p in ps.environment.sentPackets && p.src in ps.constants.config.replica_ids && p.msg.RslMessage_AppStateSupply? ==>
+           ReplyCacheObjectInv(p.msg.reply_cache, client))
+  && (forall idx :: 0 <= idx < |ps.replicas| ==> ReplyCacheObjectInv(ps.replicas[idx].replica.executor.reply_cache, client))
 }
 
 lemma lemma_ReplyCacheStateInv(
-    b:Behavior<RslState>,
-    c:LConstants,
-    i:int,
-    client:NodeIdentity
-    )
-    requires IsValidBehaviorPrefix(b, c, i);
-    requires 0 <= i;
-    ensures  ReplyCacheStateInv(b[i], client);
+  b:Behavior<RslState>,
+  c:LConstants,
+  i:int,
+  client:NodeIdentity
+  )
+  requires IsValidBehaviorPrefix(b, c, i)
+  requires 0 <= i
+  ensures  ReplyCacheStateInv(b[i], client)
 {
-    if i > 0
+  if i > 0
+  {
+    lemma_ReplyCacheStateInv(b, c, i-1, client);
+    lemma_ConstantsAllConsistent(b, c, i-1);
+    lemma_ConstantsAllConsistent(b, c, i);
+    lemma_AssumptionsMakeValidTransition(b, c, i-1);
+
+    var ps := b[i-1];
+    var ps' := b[i];
+    assert RslNext(ps, ps');
+    forall idx | 0 <= idx < |ps'.replicas|
+      ensures ReplyCacheObjectInv(ps'.replicas[idx].replica.executor.reply_cache, client)
     {
-        lemma_ReplyCacheStateInv(b, c, i-1, client);
-        lemma_ConstantsAllConsistent(b, c, i-1);
-        lemma_ConstantsAllConsistent(b, c, i);
-        lemma_AssumptionsMakeValidTransition(b, c, i-1);
+      lemma_ReplicasSize(b, c, i-1);
+      lemma_ReplicasSize(b, c, i);
 
-        var ps := b[i-1];
-        var ps' := b[i];
-        assert RslNext(ps, ps');
-        forall idx | 0 <= idx < |ps'.replicas|
-            ensures ReplyCacheObjectInv(ps'.replicas[idx].replica.executor.reply_cache, client);
+      var s := ps.replicas[idx].replica;
+      var s' := ps'.replicas[idx].replica;
+      var cache := s.executor.reply_cache;
+      var cache' := s'.executor.reply_cache;
+
+      if cache' == cache
+      {
+        assert ReplyCacheObjectInv(cache', client);
+      }
+      else
+      {
+        var ios :| RslNextOneReplica(ps, ps', idx, ios);
+        if exists inp:LPacket<NodeIdentity, RslMessage> ::
+             && LIoOpReceive(inp) in ios
+             && inp.msg.RslMessage_AppStateSupply?
+             && inp.src in s.executor.constants.all.config.replica_ids
+             && LReplicaNextProcessAppStateSupply(s, s', inp, [])
         {
-            lemma_ReplicasSize(b, c, i-1);
-            lemma_ReplicasSize(b, c, i);
-
-            var s := ps.replicas[idx].replica;
-            var s' := ps'.replicas[idx].replica;
-            var cache := s.executor.reply_cache;
-            var cache' := s'.executor.reply_cache;
-
-            if cache' == cache
-            {
-                assert ReplyCacheObjectInv(cache', client);
-            }
-            else
-            {
-                var ios :| RslNextOneReplica(ps, ps', idx, ios);
-                if exists inp ::   LIoOpReceive(inp) in ios
-                           && inp.msg.RslMessage_AppStateSupply?
-                           && inp.src in s.executor.constants.all.config.replica_ids
-                           && LReplicaNextProcessAppStateSupply(s, s', inp, [])
-                {
-                    var inp :|    LIoOpReceive(inp) in ios
-                               && inp.msg.RslMessage_AppStateSupply?
-                               && inp.src in s.executor.constants.all.config.replica_ids
-                               && LReplicaNextProcessAppStateSupply(s, s', inp, []);
-                    lemma_PacketProcessedImpliesPacketSent(ps, ps', idx, ios, inp);
-                    assert ReplyCacheObjectInv(inp.msg.reply_cache, client);
-                    assert ReplyCacheObjectInv(cache', client);
-                }
-                else
-                {
-                    assert ReplyCacheObjectInv(cache', client);
-                }
-            }
+          var inp:LPacket<NodeIdentity, RslMessage> :|
+              && LIoOpReceive(inp) in ios
+              && inp.msg.RslMessage_AppStateSupply?
+              && inp.src in s.executor.constants.all.config.replica_ids
+              && LReplicaNextProcessAppStateSupply(s, s', inp, []);
+          lemma_PacketProcessedImpliesPacketSent(ps, ps', idx, ios, inp);
+          assert ReplyCacheObjectInv(inp.msg.reply_cache, client);
+          assert ReplyCacheObjectInv(cache', client);
         }
-
-        forall p | p in ps'.environment.sentPackets && p.src in ps.constants.config.replica_ids && p.msg.RslMessage_AppStateSupply?
-            ensures ReplyCacheObjectInv(p.msg.reply_cache, client);
+        else
         {
-            if p !in ps.environment.sentPackets
-            {
-                var idx, ios := lemma_ActionThatSendsAppStateSupplyIsProcessAppStateRequest(ps, ps', p);
-            }
+          assert ReplyCacheObjectInv(cache', client);
         }
-
+      }
     }
+
+    forall p | p in ps'.environment.sentPackets && p.src in ps.constants.config.replica_ids && p.msg.RslMessage_AppStateSupply?
+      ensures ReplyCacheObjectInv(p.msg.reply_cache, client)
+    {
+      if p !in ps.environment.sentPackets
+      {
+        var idx, ios := lemma_ActionThatSendsAppStateSupplyIsProcessAppStateRequest(ps, ps', p);
+      }
+    }
+  }
 }
 
 }
