ironfleet/src/Dafny/Distributed/Protocol/RSL/Constants.i.dfy
@@ -6,17 +6,18 @@ import opened LiveRSL__Configuration_i
 import opened LiveRSL__Parameters_i
 
 datatype LConstants = LConstants(
-    config:LConfiguration,
-    params:LParameters
-    )
+  config:LConfiguration,
+  params:LParameters
+  )
 
 datatype LReplicaConstants = LReplicaConstants(
-    my_index:int,
-    all:LConstants)
+  my_index:int,
+  all:LConstants
+  )
 
 predicate LReplicaConstantsValid(c:LReplicaConstants)
 {
-    0 <= c.my_index < |c.all.config.replica_ids|
+  0 <= c.my_index < |c.all.config.replica_ids|
 }
 
 } 
