ironfleet/src/Dafny/Distributed/Protocol/RSL/Replica.i.dfy
@@ -18,358 +18,359 @@ import opened LiveRSL__Proposer_i
 import opened LiveRSL__Acceptor_i
 import opened LiveRSL__Learner_i
 import opened LiveRSL__Executor_i
+import opened LiveRSL__Broadcast_i
+import opened LiveRSL__Message_i
+import opened Common__UpperBound_s
+import opened Environment_s
 
 datatype LReplica = LReplica(
-    constants:LReplicaConstants,
-    nextHeartbeatTime:int,
-    proposer:LProposer,
-    acceptor:LAcceptor,
-    learner:LLearner,
-    executor:LExecutor)
+  constants:LReplicaConstants,
+  nextHeartbeatTime:int,
+  proposer:LProposer,
+  acceptor:LAcceptor,
+  learner:LLearner,
+  executor:LExecutor)
 
 predicate LReplicaInit(r:LReplica, c:LReplicaConstants)
-    requires WellFormedLConfiguration(c.all.config);
+  requires WellFormedLConfiguration(c.all.config)
 {
-       r.constants == c
-    && r.nextHeartbeatTime == 0
-    && LProposerInit(r.proposer, c)
-    && LAcceptorInit(r.acceptor, c)
-    && LLearnerInit(r.learner, c)
-    && LExecutorInit(r.executor, c)
+  && r.constants == c
+  && r.nextHeartbeatTime == 0
+  && LProposerInit(r.proposer, c)
+  && LAcceptorInit(r.acceptor, c)
+  && LLearnerInit(r.learner, c)
+  && LExecutorInit(r.executor, c)
 }
 
 predicate LReplicaNextProcessInvalid(s:LReplica, s':LReplica, received_packet:RslPacket, sent_packets:seq<RslPacket>)
-    requires received_packet.msg.RslMessage_Invalid?;
+  requires received_packet.msg.RslMessage_Invalid?
 {
-       s' == s
-    && sent_packets == []
+  && s' == s
+  && sent_packets == []
 }
 
 predicate LReplicaNextProcessRequest(s:LReplica, s':LReplica, received_packet:RslPacket, sent_packets:seq<RslPacket>)
-    requires received_packet.msg.RslMessage_Request?;
+  requires received_packet.msg.RslMessage_Request?
 {
-    if     received_packet.src in s.executor.reply_cache
-        && s.executor.reply_cache[received_packet.src].Reply?
-        && received_packet.msg.seqno_req <= s.executor.reply_cache[received_packet.src].seqno then
-           LExecutorProcessRequest(s.executor, received_packet, sent_packets)
-        && s' == s
-    else
-           LProposerProcessRequest(s.proposer, s'.proposer, received_packet)
-        && sent_packets == []
-        && s' == s.(proposer := s'.proposer)
+  if  && received_packet.src in s.executor.reply_cache
+      && s.executor.reply_cache[received_packet.src].Reply?
+      && received_packet.msg.seqno_req <= s.executor.reply_cache[received_packet.src].seqno then
+     && LExecutorProcessRequest(s.executor, received_packet, sent_packets)
+     && s' == s
+  else
+    && LProposerProcessRequest(s.proposer, s'.proposer, received_packet)
+    && sent_packets == []
+    && s' == s.(proposer := s'.proposer)
 }
 
 predicate LReplicaNextProcess1a(s:LReplica, s':LReplica, received_packet:RslPacket, sent_packets:seq<RslPacket>)
-    requires received_packet.msg.RslMessage_1a?;
+  requires received_packet.msg.RslMessage_1a?
 {
-       LAcceptorProcess1a(s.acceptor, s'.acceptor, received_packet, sent_packets)
-    // UNCHANGED
-    && s' == s.(acceptor := s'.acceptor)
+  && LAcceptorProcess1a(s.acceptor, s'.acceptor, received_packet, sent_packets)
+  // UNCHANGED
+  && s' == s.(acceptor := s'.acceptor)
 }
 
 predicate LReplicaNextProcess1b(s:LReplica, s':LReplica, received_packet:RslPacket, sent_packets:seq<RslPacket>)
-    requires received_packet.msg.RslMessage_1b?;
+  requires received_packet.msg.RslMessage_1b?
 {
-    if    received_packet.src in s.proposer.constants.all.config.replica_ids
-       && received_packet.msg.bal_1b == s.proposer.max_ballot_i_sent_1a
-       && s.proposer.current_state == 1
-       && (forall other_packet :: other_packet in s.proposer.received_1b_packets ==> other_packet.src != received_packet.src) then
-           LProposerProcess1b(s.proposer, s'.proposer, received_packet)
-        && LAcceptorTruncateLog(s.acceptor, s'.acceptor, received_packet.msg.log_truncation_point)
-        && sent_packets == []
-        && s' == s.(proposer := s'.proposer, acceptor := s'.acceptor)
-    else
-       s' == s && sent_packets == []
+  if  && received_packet.src in s.proposer.constants.all.config.replica_ids
+      && received_packet.msg.bal_1b == s.proposer.max_ballot_i_sent_1a
+      && s.proposer.current_state == 1
+      && (forall other_packet :: other_packet in s.proposer.received_1b_packets ==> other_packet.src != received_packet.src) then
+    && LProposerProcess1b(s.proposer, s'.proposer, received_packet)
+    && LAcceptorTruncateLog(s.acceptor, s'.acceptor, received_packet.msg.log_truncation_point)
+    && sent_packets == []
+    && s' == s.(proposer := s'.proposer, acceptor := s'.acceptor)
+  else
+    s' == s && sent_packets == []
 }
 
 predicate LReplicaNextProcessStartingPhase2(s:LReplica, s':LReplica, received_packet:RslPacket, sent_packets:seq<RslPacket>)
-    requires received_packet.msg.RslMessage_StartingPhase2?;
+  requires received_packet.msg.RslMessage_StartingPhase2?
 {
-       LExecutorProcessStartingPhase2(s.executor, s'.executor, received_packet, sent_packets)
-    && s' == s.(executor := s'.executor)
+  && LExecutorProcessStartingPhase2(s.executor, s'.executor, received_packet, sent_packets)
+  && s' == s.(executor := s'.executor)
 }
 
 predicate LReplicaNextProcess2a(s:LReplica, s':LReplica, received_packet:RslPacket, sent_packets:seq<RslPacket>)
-    requires received_packet.msg.RslMessage_2a?;
+  requires received_packet.msg.RslMessage_2a?
 {
-    var m := received_packet.msg;
-    if    received_packet.src in s.acceptor.constants.all.config.replica_ids
-       && BalLeq(s.acceptor.max_bal, m.bal_2a)
-       && LeqUpperBound(m.opn_2a, s.acceptor.constants.all.params.max_integer_val) then
-           LAcceptorProcess2a(s.acceptor, s'.acceptor, received_packet, sent_packets)
-        && s' == s.(acceptor := s'.acceptor)
-    else
-        s' == s && sent_packets == []
+  var m := received_packet.msg;
+  if  && received_packet.src in s.acceptor.constants.all.config.replica_ids
+      && BalLeq(s.acceptor.max_bal, m.bal_2a)
+      && LeqUpperBound(m.opn_2a, s.acceptor.constants.all.params.max_integer_val) then
+    && LAcceptorProcess2a(s.acceptor, s'.acceptor, received_packet, sent_packets)
+    && s' == s.(acceptor := s'.acceptor)
+  else
+    s' == s && sent_packets == []
 }
 
 predicate LReplicaNextProcess2b(s:LReplica, s':LReplica, received_packet:RslPacket, sent_packets:seq<RslPacket>)
-    requires received_packet.msg.RslMessage_2b?;
+  requires received_packet.msg.RslMessage_2b?
 {
-    var opn := received_packet.msg.opn_2b;
-    var op_learnable := s.executor.ops_complete < opn || (s.executor.ops_complete == opn && s.executor.next_op_to_execute.OutstandingOpUnknown?);
-    if op_learnable then
-           LLearnerProcess2b(s.learner, s'.learner, received_packet)
-        && sent_packets == []
-        && s' == s.(learner := s'.learner)
-    else
-           s' == s
-        && sent_packets == []
+  var opn := received_packet.msg.opn_2b;
+  var op_learnable := s.executor.ops_complete < opn || (s.executor.ops_complete == opn && s.executor.next_op_to_execute.OutstandingOpUnknown?);
+  if op_learnable then
+    && LLearnerProcess2b(s.learner, s'.learner, received_packet)
+    && sent_packets == []
+    && s' == s.(learner := s'.learner)
+  else
+    && s' == s
+    && sent_packets == []
 }
 
 predicate LReplicaNextProcessReply(s:LReplica, s':LReplica, received_packet:RslPacket, sent_packets:seq<RslPacket>)
-    requires received_packet.msg.RslMessage_Reply?;
+  requires received_packet.msg.RslMessage_Reply?
 {
-       sent_packets == []
-    && s' == s
+  && sent_packets == []
+  && s' == s
 }
 
 predicate LReplicaNextProcessAppStateSupply(s:LReplica, s':LReplica, received_packet:RslPacket, sent_packets:seq<RslPacket>)
-    requires received_packet.msg.RslMessage_AppStateSupply?;
+  requires received_packet.msg.RslMessage_AppStateSupply?
 {
-    if received_packet.src in s.executor.constants.all.config.replica_ids && received_packet.msg.opn_state_supply > s.executor.ops_complete then
-           LLearnerForgetOperationsBefore(s.learner, s'.learner, received_packet.msg.opn_state_supply)
-        && LExecutorProcessAppStateSupply(s.executor, s'.executor, received_packet)
-        && sent_packets == []
-        && s' == s.(learner := s'.learner, executor := s'.executor)
-    else
-        s' == s && sent_packets == []
+  if received_packet.src in s.executor.constants.all.config.replica_ids && received_packet.msg.opn_state_supply > s.executor.ops_complete then
+    && LLearnerForgetOperationsBefore(s.learner, s'.learner, received_packet.msg.opn_state_supply)
+    && LExecutorProcessAppStateSupply(s.executor, s'.executor, received_packet)
+    && sent_packets == []
+    && s' == s.(learner := s'.learner, executor := s'.executor)
+  else
+    s' == s && sent_packets == []
 }
 
 predicate LReplicaNextProcessAppStateRequest(s:LReplica, s':LReplica, received_packet:RslPacket, sent_packets:seq<RslPacket>)
-    requires received_packet.msg.RslMessage_AppStateRequest?;
+  requires received_packet.msg.RslMessage_AppStateRequest?
 {
-       LExecutorProcessAppStateRequest(s.executor, s'.executor, received_packet, sent_packets)
-    && s' == s.(executor := s'.executor)
+  && LExecutorProcessAppStateRequest(s.executor, s'.executor, received_packet, sent_packets)
+  && s' == s.(executor := s'.executor)
 }
 
 predicate LReplicaNextProcessHeartbeat(s:LReplica, s':LReplica, received_packet:RslPacket, clock:int, sent_packets:seq<RslPacket>)
-    requires received_packet.msg.RslMessage_Heartbeat?;
+  requires received_packet.msg.RslMessage_Heartbeat?
 {
-       LProposerProcessHeartbeat(s.proposer, s'.proposer, received_packet, clock)
-    && LAcceptorProcessHeartbeat(s.acceptor, s'.acceptor, received_packet)
-    && sent_packets == []
-    && s' == s.(proposer := s'.proposer, acceptor := s'.acceptor)
+  && LProposerProcessHeartbeat(s.proposer, s'.proposer, received_packet, clock)
+  && LAcceptorProcessHeartbeat(s.acceptor, s'.acceptor, received_packet)
+  && sent_packets == []
+  && s' == s.(proposer := s'.proposer, acceptor := s'.acceptor)
 }
 
 predicate LReplicaNextSpontaneousMaybeEnterNewViewAndSend1a(s:LReplica, s':LReplica, sent_packets:seq<RslPacket>)
 {
-       LProposerMaybeEnterNewViewAndSend1a(s.proposer, s'.proposer, sent_packets)
-    && s' == s.(proposer := s'.proposer)
+  && LProposerMaybeEnterNewViewAndSend1a(s.proposer, s'.proposer, sent_packets)
+  && s' == s.(proposer := s'.proposer)
 }
 
 predicate LReplicaNextSpontaneousMaybeEnterPhase2(s:LReplica, s':LReplica, sent_packets:seq<RslPacket>)
 {
-       LProposerMaybeEnterPhase2(s.proposer, s'.proposer, s.acceptor.log_truncation_point, sent_packets)
-    && s' == s.(proposer := s'.proposer)
+  && LProposerMaybeEnterPhase2(s.proposer, s'.proposer, s.acceptor.log_truncation_point, sent_packets)
+  && s' == s.(proposer := s'.proposer)
 }
 
 predicate LReplicaNextReadClockMaybeNominateValueAndSend2a(s:LReplica, s':LReplica, clock:ClockReading, sent_packets:seq<RslPacket>)
 {
-       LProposerMaybeNominateValueAndSend2a(s.proposer, s'.proposer, clock.t, s.acceptor.log_truncation_point, sent_packets)
-    && s' == s.(proposer := s'.proposer)
+  && LProposerMaybeNominateValueAndSend2a(s.proposer, s'.proposer, clock.t, s.acceptor.log_truncation_point, sent_packets)
+  && s' == s.(proposer := s'.proposer)
 }
 
 predicate LReplicaNextSpontaneousTruncateLogBasedOnCheckpoints(s:LReplica, s':LReplica, sent_packets:seq<RslPacket>)
 {
-    (exists opn ::
-           IsLogTruncationPointValid(opn, s.acceptor.last_checkpointed_operation, s.constants.all.config)
+  (exists opn ::
+        && IsLogTruncationPointValid(opn, s.acceptor.last_checkpointed_operation, s.constants.all.config)
         && opn > s.acceptor.log_truncation_point
         && LAcceptorTruncateLog(s.acceptor, s'.acceptor, opn)
         && s' == s.(acceptor := s'.acceptor)
         && sent_packets == []
-    )
-    ||
-    (exists opn ::
-           IsLogTruncationPointValid(opn, s.acceptor.last_checkpointed_operation, s.constants.all.config)
+  )
+  ||
+  (exists opn ::
+        && IsLogTruncationPointValid(opn, s.acceptor.last_checkpointed_operation, s.constants.all.config)
         && opn <= s.acceptor.log_truncation_point
         && s' == s
         && sent_packets == []
-    )
+  )
 }
 
 predicate LReplicaNextSpontaneousMaybeMakeDecision(s:LReplica, s':LReplica, sent_packets:seq<RslPacket>)
 {
-    var opn := s.executor.ops_complete;
-    if    s.executor.next_op_to_execute.OutstandingOpUnknown?
-       && opn in s.learner.unexecuted_learner_state
-       && |s.learner.unexecuted_learner_state[opn].received_2b_message_senders| >= LMinQuorumSize(s.learner.constants.all.config) then
-           LExecutorGetDecision(s.executor, s'.executor, s.learner.max_ballot_seen, opn, s.learner.unexecuted_learner_state[opn].candidate_learned_value)
-        && s' == s.(executor := s'.executor)
-        && sent_packets == []
-    else
-        s' == s && sent_packets == []
+  var opn := s.executor.ops_complete;
+  if  && s.executor.next_op_to_execute.OutstandingOpUnknown?
+      && opn in s.learner.unexecuted_learner_state
+      && |s.learner.unexecuted_learner_state[opn].received_2b_message_senders| >= LMinQuorumSize(s.learner.constants.all.config) then
+    && LExecutorGetDecision(s.executor, s'.executor, s.learner.max_ballot_seen, opn,
+                           s.learner.unexecuted_learner_state[opn].candidate_learned_value)
+    && s' == s.(executor := s'.executor)
+    && sent_packets == []
+  else
+    s' == s && sent_packets == []
 }
 
 predicate LReplicaNextSpontaneousMaybeExecute(s:LReplica, s':LReplica, sent_packets:seq<RslPacket>)
 {
-    if    s.executor.next_op_to_execute.OutstandingOpKnown?
-        && LtUpperBound(s.executor.ops_complete, s.executor.constants.all.params.max_integer_val)
-        && LReplicaConstantsValid(s.executor.constants) then
-        var v := s.executor.next_op_to_execute.v;
-           LProposerResetViewTimerDueToExecution(s.proposer, s'.proposer, v)
-        && LLearnerForgetDecision(s.learner, s'.learner, s.executor.ops_complete)
-        && LExecutorExecute(s.executor, s'.executor, sent_packets)
-        && s' == s.(proposer := s'.proposer, learner := s'.learner, executor := s'.executor)
-    else
-        s' == s && sent_packets == []
+  if  && s.executor.next_op_to_execute.OutstandingOpKnown?
+      && LtUpperBound(s.executor.ops_complete, s.executor.constants.all.params.max_integer_val)
+      && LReplicaConstantsValid(s.executor.constants) then
+    var v := s.executor.next_op_to_execute.v;
+    && LProposerResetViewTimerDueToExecution(s.proposer, s'.proposer, v)
+    && LLearnerForgetDecision(s.learner, s'.learner, s.executor.ops_complete)
+    && LExecutorExecute(s.executor, s'.executor, sent_packets)
+    && s' == s.(proposer := s'.proposer, learner := s'.learner, executor := s'.executor)
+  else
+    s' == s && sent_packets == []
 }
 
 predicate LReplicaNextReadClockMaybeSendHeartbeat(s:LReplica, s':LReplica, clock:ClockReading, sent_packets:seq<RslPacket>)
 {
-    if clock.t < s.nextHeartbeatTime then
-        s' == s && sent_packets == []
-    else
-           s'.nextHeartbeatTime == UpperBoundedAddition(clock.t, s.constants.all.params.heartbeat_period, s.constants.all.params.max_integer_val)
-        && LBroadcastToEveryone(s.constants.all.config, s.constants.my_index,
-                                RslMessage_Heartbeat(s.proposer.election_state.current_view,
-                                                        s.constants.my_index in s.proposer.election_state.current_view_suspectors,
-                                                        s.executor.ops_complete),
-                                sent_packets)
-        && s' == s.(nextHeartbeatTime := s'.nextHeartbeatTime)
+  if clock.t < s.nextHeartbeatTime then
+    s' == s && sent_packets == []
+  else
+    && s'.nextHeartbeatTime == UpperBoundedAddition(clock.t, s.constants.all.params.heartbeat_period, s.constants.all.params.max_integer_val)
+    && LBroadcastToEveryone(s.constants.all.config, s.constants.my_index,
+                           RslMessage_Heartbeat(s.proposer.election_state.current_view,
+                                                s.constants.my_index in s.proposer.election_state.current_view_suspectors,
+                                                s.executor.ops_complete),
+                           sent_packets)
+    && s' == s.(nextHeartbeatTime := s'.nextHeartbeatTime)
 }
 
 predicate LReplicaNextReadClockCheckForViewTimeout(s:LReplica, s':LReplica, clock:ClockReading, sent_packets:seq<RslPacket>)
 {
-      LProposerCheckForViewTimeout(s.proposer, s'.proposer, clock.t)
-   && sent_packets == []
-   && s' == s.(proposer := s'.proposer)
+  && LProposerCheckForViewTimeout(s.proposer, s'.proposer, clock.t)
+  && sent_packets == []
+  && s' == s.(proposer := s'.proposer)
 }
 
 predicate LReplicaNextReadClockCheckForQuorumOfViewSuspicions(s:LReplica, s':LReplica, clock:ClockReading, sent_packets:seq<RslPacket>)
 {
-       LProposerCheckForQuorumOfViewSuspicions(s.proposer, s'.proposer, clock.t)
-    && sent_packets == []
-    && s' == s.(proposer := s'.proposer)
+  && LProposerCheckForQuorumOfViewSuspicions(s.proposer, s'.proposer, clock.t)
+  && sent_packets == []
+  && s' == s.(proposer := s'.proposer)
 }
 
 function {:opaque} ExtractSentPacketsFromIos(ios:seq<RslIo>) : seq<RslPacket>
-    ensures forall p :: p in ExtractSentPacketsFromIos(ios) <==> LIoOpSend(p) in ios;
+  ensures forall p :: p in ExtractSentPacketsFromIos(ios) <==> LIoOpSend(p) in ios
 {
-    if |ios| == 0 then
-        []
-    else if ios[0].LIoOpSend? then
-        [ios[0].s] + ExtractSentPacketsFromIos(ios[1..])
-    else
-        ExtractSentPacketsFromIos(ios[1..])
+  if |ios| == 0 then
+    []
+  else if ios[0].LIoOpSend? then
+    [ios[0].s] + ExtractSentPacketsFromIos(ios[1..])
+  else
+    ExtractSentPacketsFromIos(ios[1..])
 }
 
 predicate LReplicaNextReadClockAndProcessPacket(s:LReplica, s':LReplica, ios:seq<RslIo>)
-    requires |ios| >= 1;
-    requires ios[0].LIoOpReceive?;
-    requires ios[0].r.msg.RslMessage_Heartbeat?;
+  requires |ios| >= 1
+  requires ios[0].LIoOpReceive?
+  requires ios[0].r.msg.RslMessage_Heartbeat?
 {
-       |ios| > 1
-    && ios[1].LIoOpReadClock?
-    && (forall io :: io in ios[2..] ==> io.LIoOpSend?)
-    && LReplicaNextProcessHeartbeat(s, s', ios[0].r, ios[1].t, ExtractSentPacketsFromIos(ios))
+  && |ios| > 1
+  && ios[1].LIoOpReadClock?
+  && (forall io :: io in ios[2..] ==> io.LIoOpSend?)
+  && LReplicaNextProcessHeartbeat(s, s', ios[0].r, ios[1].t, ExtractSentPacketsFromIos(ios))
 }
 
 predicate LReplicaNextProcessPacketWithoutReadingClock(s:LReplica, s':LReplica, ios:seq<RslIo>)
-    requires |ios| >= 1;
-    requires ios[0].LIoOpReceive?;
-    requires !ios[0].r.msg.RslMessage_Heartbeat?;
+  requires |ios| >= 1
+  requires ios[0].LIoOpReceive?
+  requires !ios[0].r.msg.RslMessage_Heartbeat?
 {
-       (forall io :: io in ios[1..] ==> io.LIoOpSend?)
-    && var sent_packets := ExtractSentPacketsFromIos(ios);
-       (match ios[0].r.msg
-            case RslMessage_Invalid => LReplicaNextProcessInvalid(s, s', ios[0].r, sent_packets)
-            case RslMessage_Request(_, _) => LReplicaNextProcessRequest(s, s', ios[0].r, sent_packets)
-            case RslMessage_1a(_) => LReplicaNextProcess1a(s, s', ios[0].r, sent_packets)
-            case RslMessage_1b(_, _, _) => LReplicaNextProcess1b(s, s', ios[0].r, sent_packets)
-            case RslMessage_StartingPhase2(_, _) => LReplicaNextProcessStartingPhase2(s, s', ios[0].r, sent_packets)
-            case RslMessage_2a(_, _, _) => LReplicaNextProcess2a(s, s', ios[0].r, sent_packets)
-            case RslMessage_2b(_, _, _) => LReplicaNextProcess2b(s, s', ios[0].r, sent_packets)
-            case RslMessage_Reply(_, _) => LReplicaNextProcessReply(s, s', ios[0].r, sent_packets)
-            case RslMessage_AppStateRequest(_, _) => LReplicaNextProcessAppStateRequest(s, s', ios[0].r, sent_packets)
-            case RslMessage_AppStateSupply(_, _, _, _) => LReplicaNextProcessAppStateSupply(s, s', ios[0].r, sent_packets)
-      )
+  && (forall io :: io in ios[1..] ==> io.LIoOpSend?)
+  && var sent_packets := ExtractSentPacketsFromIos(ios);
+    match ios[0].r.msg
+       case RslMessage_Invalid => LReplicaNextProcessInvalid(s, s', ios[0].r, sent_packets)
+       case RslMessage_Request(_, _) => LReplicaNextProcessRequest(s, s', ios[0].r, sent_packets)
+       case RslMessage_1a(_) => LReplicaNextProcess1a(s, s', ios[0].r, sent_packets)
+       case RslMessage_1b(_, _, _) => LReplicaNextProcess1b(s, s', ios[0].r, sent_packets)
+       case RslMessage_StartingPhase2(_, _) => LReplicaNextProcessStartingPhase2(s, s', ios[0].r, sent_packets)
+       case RslMessage_2a(_, _, _) => LReplicaNextProcess2a(s, s', ios[0].r, sent_packets)
+       case RslMessage_2b(_, _, _) => LReplicaNextProcess2b(s, s', ios[0].r, sent_packets)
+       case RslMessage_Reply(_, _) => LReplicaNextProcessReply(s, s', ios[0].r, sent_packets)
+       case RslMessage_AppStateRequest(_, _) => LReplicaNextProcessAppStateRequest(s, s', ios[0].r, sent_packets)
+       case RslMessage_AppStateSupply(_, _, _, _) => LReplicaNextProcessAppStateSupply(s, s', ios[0].r, sent_packets)
 }
 
 predicate LReplicaNextProcessPacket(s:LReplica, s':LReplica, ios:seq<RslIo>)
 {
-       |ios| >= 1
-    && if ios[0].LIoOpTimeoutReceive? then
-           s' == s && |ios| == 1
-       else
-       (
-              ios[0].LIoOpReceive?
-           && if ios[0].r.msg.RslMessage_Heartbeat? then
-                  LReplicaNextReadClockAndProcessPacket(s, s', ios)
-              else
-                  LReplicaNextProcessPacketWithoutReadingClock(s, s', ios)
-       )
+  && |ios| >= 1
+  && if ios[0].LIoOpTimeoutReceive? then
+      s' == s && |ios| == 1
+    else
+      (&& ios[0].LIoOpReceive?
+       && if ios[0].r.msg.RslMessage_Heartbeat? then
+           LReplicaNextReadClockAndProcessPacket(s, s', ios)
+         else
+           LReplicaNextProcessPacketWithoutReadingClock(s, s', ios)
+      )
 }
 
 function LReplicaNumActions() : int
 {
-    10
+  10
 }
 
 predicate SpontaneousIos(ios:seq<RslIo>, clocks:int)
-    requires 0<=clocks<=1;
+  requires 0<=clocks<=1
 {
-       clocks <= |ios|
-    && (forall i :: 0<=i<clocks ==> ios[i].LIoOpReadClock?)
-    && (forall i :: clocks<=i<|ios| ==> ios[i].LIoOpSend?)
+  && clocks <= |ios|
+  && (forall i :: 0<=i<clocks ==> ios[i].LIoOpReadClock?)
+  && (forall i :: clocks<=i<|ios| ==> ios[i].LIoOpSend?)
 }
 
 function SpontaneousClock(ios:seq<RslIo>) : ClockReading
 {
-    if SpontaneousIos(ios, 1)
-        then ClockReading(ios[0].t)
-        else ClockReading(0)  // nonsense to avoid putting a precondition on this function
+  if SpontaneousIos(ios, 1) then ClockReading(ios[0].t) else ClockReading(0) // nonsense to avoid putting a precondition on this function
 }
 
 predicate LReplicaNoReceiveNext(s:LReplica, nextActionIndex:int, s':LReplica, ios:seq<RslIo>)
 {
-    var sent_packets := ExtractSentPacketsFromIos(ios);
+  var sent_packets := ExtractSentPacketsFromIos(ios);
 
-    if nextActionIndex == 1 then
-           SpontaneousIos(ios, 0)
-        && LReplicaNextSpontaneousMaybeEnterNewViewAndSend1a(s, s', sent_packets)
-    else if nextActionIndex == 2 then
-           SpontaneousIos(ios, 0)
-        && LReplicaNextSpontaneousMaybeEnterPhase2(s, s', sent_packets)
-    else if nextActionIndex == 3 then
-           SpontaneousIos(ios, 1)
-        && LReplicaNextReadClockMaybeNominateValueAndSend2a(s, s', SpontaneousClock(ios), sent_packets)
-    else if nextActionIndex == 4 then
-           SpontaneousIos(ios, 0)
-        && LReplicaNextSpontaneousTruncateLogBasedOnCheckpoints(s, s', sent_packets)
-    else if nextActionIndex == 5 then
-           SpontaneousIos(ios, 0)
-        && LReplicaNextSpontaneousMaybeMakeDecision(s, s', sent_packets)
-    else if nextActionIndex == 6 then
-           SpontaneousIos(ios, 0)
-        && LReplicaNextSpontaneousMaybeExecute(s, s', sent_packets)
-    else if nextActionIndex == 7 then
-           SpontaneousIos(ios, 1)
-        && LReplicaNextReadClockCheckForViewTimeout(s, s', SpontaneousClock(ios), sent_packets)
-    else if nextActionIndex == 8 then
-           SpontaneousIos(ios, 1)
-        && LReplicaNextReadClockCheckForQuorumOfViewSuspicions(s, s', SpontaneousClock(ios), sent_packets)
-    else
-           nextActionIndex == 9
-        && SpontaneousIos(ios, 1)
-        && LReplicaNextReadClockMaybeSendHeartbeat(s, s', SpontaneousClock(ios), sent_packets)
+  if nextActionIndex == 1 then
+    && SpontaneousIos(ios, 0)
+    && LReplicaNextSpontaneousMaybeEnterNewViewAndSend1a(s, s', sent_packets)
+  else if nextActionIndex == 2 then
+    && SpontaneousIos(ios, 0)
+    && LReplicaNextSpontaneousMaybeEnterPhase2(s, s', sent_packets)
+  else if nextActionIndex == 3 then
+    && SpontaneousIos(ios, 1)
+    && LReplicaNextReadClockMaybeNominateValueAndSend2a(s, s', SpontaneousClock(ios), sent_packets)
+  else if nextActionIndex == 4 then
+    && SpontaneousIos(ios, 0)
+    && LReplicaNextSpontaneousTruncateLogBasedOnCheckpoints(s, s', sent_packets)
+  else if nextActionIndex == 5 then
+    && SpontaneousIos(ios, 0)
+    && LReplicaNextSpontaneousMaybeMakeDecision(s, s', sent_packets)
+  else if nextActionIndex == 6 then
+    && SpontaneousIos(ios, 0)
+    && LReplicaNextSpontaneousMaybeExecute(s, s', sent_packets)
+  else if nextActionIndex == 7 then
+    && SpontaneousIos(ios, 1)
+    && LReplicaNextReadClockCheckForViewTimeout(s, s', SpontaneousClock(ios), sent_packets)
+  else if nextActionIndex == 8 then
+    && SpontaneousIos(ios, 1)
+    && LReplicaNextReadClockCheckForQuorumOfViewSuspicions(s, s', SpontaneousClock(ios), sent_packets)
+  else
+    && nextActionIndex == 9
+    && SpontaneousIos(ios, 1)
+    && LReplicaNextReadClockMaybeSendHeartbeat(s, s', SpontaneousClock(ios), sent_packets)
 }
 
 datatype LScheduler = LScheduler(replica:LReplica, nextActionIndex:int)
 
 predicate LSchedulerInit(s:LScheduler, c:LReplicaConstants)
-    requires WellFormedLConfiguration(c.all.config);
+  requires WellFormedLConfiguration(c.all.config)
 {
-       LReplicaInit(s.replica, c)
-    && s.nextActionIndex == 0
+  && LReplicaInit(s.replica, c)
+  && s.nextActionIndex == 0
 }
 
 predicate LSchedulerNext(s:LScheduler, s':LScheduler, ios:seq<RslIo>)
 {
-       s'.nextActionIndex == (s.nextActionIndex + 1) % LReplicaNumActions()
-    && if s.nextActionIndex == 0 then
-          LReplicaNextProcessPacket(s.replica, s'.replica, ios)
-       else
-           LReplicaNoReceiveNext(s.replica, s.nextActionIndex, s'.replica, ios)
+  && s'.nextActionIndex == (s.nextActionIndex + 1) % LReplicaNumActions()
+  && if s.nextActionIndex == 0 then
+      LReplicaNextProcessPacket(s.replica, s'.replica, ios)
+    else
+      LReplicaNoReceiveNext(s.replica, s.nextActionIndex, s'.replica, ios)
 }
 
 } 
