ironfleet/src/Dafny/Distributed/Services/RSL/RSLDistributedSystem.i.dfy
@@ -2,7 +2,5 @@ include "../../Impl/RSL/Host.i.dfy"
 include "../../Common/Framework/DistributedSystem.s.dfy"
 
 module RSL_DistributedSystem_i refines DistributedSystem_s {
-
-    import opened H_s = Host_i
-
+  import opened H_s = Host_i
 }
